Implementing map with proofs, correctly
Add list instead of single element
Add invariants: not null, nodups, all have consistent keys
Proving correct operations: did add, remove, merge
Need to clean up merge proofs

src/util/extmap.v
@@ -160,6 +160,16 @@ Parameter map_inj_eq: forall {A B: Type} (f: A -> B) (m1 m2: t A)
 Parameter find_opt_contains: forall {a: Type} (m: t a) (k: key),
   contains m k = isSome (find_opt k m).
 
+(*Our specifications will be in terms of [find_opt]*)
+Parameter find_opt_inter: forall {a b c: Type} (f: key -> a -> b -> option c) (m1: t a) (m2: t b)
+  (k: key) (v: c),
+  find_opt k (inter f m1 m2) = Some v <-> 
+  exists v1 v2, find_opt k m1 = Some v1 /\ find_opt k m2 = Some v2 /\ f k v1 v2 = Some v.
+
+Parameter find_opt_set_inter: forall {a: Type} (m1 m2: t a) (k: key) (v: a),
+  find_opt k (set_inter m1 m2) = Some v <->
+  find_opt k m1 = Some v /\ exists v2, find_opt k m2 = Some v2.
+
 End S.
 
 
@@ -171,6 +181,14 @@ Parameter tag: t -> CoqBigInt.t.
 (*We do not yet require this to be decidable equality;
   we only require that when used*)
 Parameter equal : t -> t -> bool.
+(*But we do need that equality implies equal tags (NOTE that
+the equality is NOT always structural; e.g. alpha equivalence)
+But it MUST be compatible with tags*)
+(*It must be transitive*)
+Parameter eq_refl: forall t, equal t t.
+Parameter eq_sym: forall t1 t2, equal t1 t2 = equal t2 t1.
+Parameter eq_trans: forall t1 t2 t3, equal t1 t2 -> equal t2 t3 -> equal t1 t3.
+Parameter eq_compat: forall t1 t2, equal t1 t2 -> tag t1 = tag t2.
 End TaggedType.
 
 Module Make (T: TaggedType) <: S.
@@ -184,39 +202,174 @@ Definition tag x := CoqBigInt.to_Z (T.tag x).
 Local Instance key_count : Countable key :=
   Build_Countable T.t key_eq T.tag T.untag T.tag_untag.*)
 
+(*TODO: move*)
+(*NOTE: arbitrary equality predicate*)
+Section ListEqGen.
+Context {A: Type} (eq: A -> A -> bool).
+
+Definition inb (x: A) (l: list A) : bool :=
+  existsb (eq x) l.
+
+Fixpoint uniq (l: list A) : bool :=
+  match l with
+  | x :: xs => negb (inb x xs) && uniq xs
+  | nil => true
+  end.
+
+Definition unionb (l1 l2: list A) : list A :=
+  fold_right (fun x acc => if inb x acc then acc else x :: acc) l2 l1.
+
+Lemma uniq_unionb (l1 l2: list A):
+  uniq l2 ->
+  uniq (unionb l1 l2).
+Proof.
+  induction l1 as [| h t IH]; simpl; auto.
+  intros Huniq.
+  destruct (inb h (unionb t l2)) eqn : Hinb; auto.
+  simpl. rewrite Hinb. auto.
+Qed.
+
+Variable (eq_refl: forall x, eq x x).
+Variable (eq_sym: forall x y, eq x y = eq y x).
+Variable (eq_trans: forall x y z, eq x y -> eq y z -> eq x z).
+
+Lemma inb_congr (l: list A) (x1 x2: A):
+  eq x1 x2 ->
+  inb x1 l = inb x2 l.
+Proof.
+  intros Heq. induction l as [| h1 t1 IH]; simpl; auto.
+  rewrite IH. f_equal.
+  destruct (eq x1 h1) eqn : Heq1; destruct (eq x2 h1) eqn : Heq2; auto.
+  - rewrite <- Heq2. symmetry. apply (eq_trans x2 x1 h1); auto.
+    rewrite eq_sym; auto.
+  - rewrite <- Heq1. apply (eq_trans x1 x2 h1); auto.
+Qed.
+
+Lemma inb_unionb (l1 l2: list A) (x: A):
+  inb x (unionb l1 l2) = inb x l1 || inb x l2.
+Proof.
+  revert x.
+  induction l1 as [| h1 t1 IH]; simpl; auto. intros x.
+  destruct (inb h1 (unionb t1 l2)) eqn : Hin; simpl; rewrite IH; auto.
+  - rewrite IH in Hin. 
+    destruct (eq x h1) eqn : Heq; auto.
+    simpl. rewrite !(inb_congr _ _ _ Heq). auto.
+  - rewrite orb_assoc. reflexivity.
+Qed. 
+
+Lemma inb_filter (p: A -> bool) (Hp: forall x y, eq x y -> p x -> p y) (x: A) (l: list A):
+  inb x (List.filter p l) = inb x l && p x.
+Proof.
+  induction l as [| h t IH]; simpl; auto.
+  destruct (p h) eqn : Hph.
+  - simpl. rewrite IH, andb_orb_distrib_l.
+    destruct (eq x h) eqn : Heq; simpl; auto.
+    rewrite eq_sym in Heq.
+    apply Hp in Heq; auto. rewrite Heq. auto.
+  - rewrite IH. destruct (eq x h) eqn : Heq; simpl; auto.
+    destruct (p x) eqn : Hpx; auto; [| rewrite andb_false_r; auto].
+    assert (Hph2: p h = true) by (apply (Hp x); auto).
+    rewrite Hph2 in Hph; discriminate.
+Qed.
+
+(*Unconditionally, anything in filter is in the original list*)
+Lemma inb_filter_in (p: A -> bool) (x: A) (l: list A):
+  inb x (List.filter p l) -> inb x l.
+Proof.
+  induction l as [| h t IH]; simpl; auto.
+  destruct (p h); simpl; auto.
+  - apply orb_impl_l; auto.
+  - intros Hin. apply IH in Hin; rewrite Hin, orb_true_r. auto.
+Qed. 
+
+Lemma uniq_filter (p: A -> bool) l:
+  uniq l ->
+  uniq (List.filter p l).
+Proof.
+  induction l as [| h t IH]; simpl; auto.
+  intros Hinu. apply andb_true_iff in Hinu. destruct Hinu as [Hnotin Hu].
+  destruct (p h) eqn : Hph; simpl; auto.
+  destruct (inb h (List.filter p t)) eqn : Hinf; simpl; auto.
+  apply inb_filter_in in Hinf. rewrite Hinf in Hnotin. discriminate.
+Qed.
+
+Lemma inb_In x l:
+  inb x l ->
+  exists y, In y l /\ eq x y.
+Proof.
+  induction l as [| h1 t1 IH]; simpl; auto; [discriminate|].
+  destruct (eq x h1) eqn : Hx; simpl.
+  - intros _. exists h1. auto.
+  - intros Hin. apply IH in Hin. destruct_all; eauto.
+Qed.
+
+Lemma In_inb x l:
+  In x l ->
+  inb x l.
+Proof.
+  induction l as [| h1 t1 IH]; simpl; auto.
+  intros [Heq | Hin]; subst; auto.
+  - rewrite eq_refl. auto.
+  - rewrite IH, orb_true_r; auto.
+Qed.
+
+End ListEqGen.
+
+
 (*Union, merge, etc need to know key for function, so 
   we store it as well. We could modify gmap, maybe we will
   do that later*)
 (*For proofs of canonicity, we need to know this invariant, so
   we need a sigma type*)
-Definition gmap_wf {A: Type} (g: Zmap (key * A)) : bool :=
-  map_fold (fun k v acc => Z.eqb k 
-    (tag (fst v)) && acc) true g.
+Definition gmap_wf {A: Type} (g: Zmap (list (key * A))) : bool :=
+  map_fold (fun k (v: list (key * A)) acc => negb (Common.null v) && 
+    uniq T.equal (map fst v) &&
+    (forallb (Z.eqb k) (map tag (map fst v)) && acc)) true g.
 
 Lemma and_true_r (P: Prop) : P <-> P /\ true.
 Proof.
   split; auto. intros [Hp]; auto.
 Qed.
 
+Lemma and_iff_compat {P1 P2 P3 P4: Prop}:
+  P1 <-> P3 ->
+  P2 <-> P4 ->
+  P1 /\ P2 <-> P3 /\ P4.
+Proof.
+  intros. tauto.
+Qed.
+
 (*Rewrite in terms of Map_forall*)
-Lemma gmap_wf_iff {A: Type} (g: Zmap (key * A)):
-  gmap_wf g <-> map_Forall (fun k v => k =tag (fst v)) g.
+Lemma gmap_wf_iff {A: Type} (g: Zmap (list (key * A))):
+  gmap_wf g <-> map_Forall (fun k v => v <> nil /\ uniq T.equal (map fst v) /\ 
+    Forall (fun x => k = tag (fst x)) v) g. 
 Proof.
   unfold gmap_wf.
   apply (map_fold_ind (fun r m =>
-    is_true r <-> map_Forall (fun k (v: key * A) => k = tag (fst v)) m
+    is_true r <-> map_Forall (fun k v => v <> nil /\ uniq T.equal (map fst v) /\ 
+    Forall (fun x => k = tag (fst x)) v) m
   )).
   - split; auto. intros. apply map_Forall_empty.
   - intros k v m b Hnot Hb.
     unfold is_true.
-    rewrite andb_true_iff, Hb, map_Forall_insert; auto.
-    apply and_iff_compat_r.
-    destruct (Z.eqb_spec k (tag v.1)); subst; simpl; split; auto; discriminate.
-Qed.
+    rewrite !andb_true_iff, Hb, map_Forall_insert; auto. rewrite !Logic.and_assoc.
+    apply and_iff_compat.
+    { destruct v; simpl; split; auto. }
+    apply and_iff_compat; auto.
+    apply and_iff_compat; auto.
+    rewrite map_map, forallb_map.
+    clear. induction v; simpl; auto; [split; auto |].
+    rewrite andb_true_iff.
+    split.
+    + intros [Hkeq Hall]. apply Z.eqb_eq in Hkeq. subst. 
+      constructor; auto. apply IHv; auto.
+    + intros Hall. inversion Hall; subst; auto. rewrite Z.eqb_refl. split; auto.
+      apply IHv; auto.
+Qed. 
 
-Definition t (A: Type) : Type := { g : Zmap (key * A) | gmap_wf g}.
+Definition t (A: Type) : Type := { g : Zmap (list (key * A)) | gmap_wf g}.
 
-Definition mp {A: Type} (m: t A) : Zmap (key * A) := proj1_sig m.
+Definition mp {A: Type} (m: t A) : Zmap (list (key * A)) := proj1_sig m.
 
 Section Types.
 
@@ -233,104 +386,802 @@ Definition is_empty (m: t a): bool :=
   | _, _, _ => false
   end.
 
-Definition mem (k: key) (m: t a) : bool :=
-  match (mp m) !! tag k with
-  | None => false
-  | Some _ => true
-  end.
+  (*TODO: import AssocList?*)
+(*NOTE: this is generic boolean eq, not eq_dec*)
+Definition get_list {A: Type} (k: key) (l: list (key * A)) : option A :=
+  option_map snd (find (fun x => T.equal k (fst x)) l).
 
-Lemma add_wf {A: Type} (k: key) (v: A) (m: t A) :
-  gmap_wf (<[tag k:=(k, v)]> (mp m)).
+(*Because Coq is terrible at unifying things*)
+Ltac destruct_if Heq := match goal with |- context [(if ?b then ?x else ?y)] => destruct b eqn : Heq
+    end.
+
+Lemma get_list_cons {A: Type} (k: key) (x: key * A) (t: list (key * A)) :
+  get_list k (x :: t) = if T.equal k (fst x) then Some (snd x) else get_list k t.
 Proof.
-  apply gmap_wf_iff.
-  apply map_Forall_insert_2; auto.
-  destruct m; apply gmap_wf_iff; auto.
+  unfold get_list; simpl. unfold key in *.
+  destruct (T.equal k x.1); auto.
 Qed.
 
+Lemma get_list_nil {A: Type} (k: key):
+  @get_list A k nil = None.
+Proof. reflexivity. Qed.
+
+(*Problem: what if first doesnt satisfy p*)
+Lemma find_filter {A: Type} (p: A -> bool) (p1: A -> bool) (l: list A):
+  find p1 (List.filter p l) = 
+  find (fun x => p1 x && p x) l.
+Proof.
+  induction l as [| h1 t1 IH]; simpl; auto.
+  destruct (p h1) eqn : Hph1; simpl; auto.
+  + destruct (p1 h1) eqn : Hp1h1; auto.
+  + rewrite andb_false_r. auto.
+Qed.
+
+Definition remove_list {A: Type} (k: key) (l: list (key * A)) : list (key * A) :=
+  List.filter (fun x => negb (T.equal k (fst x))) l.
+
+(*TODO: did I prove?*)
+Lemma filter_sublist {A: Type} (p: A -> bool) (l: list A):
+  Common.sublist (List.filter p l) l.
+Proof.
+  intros x. rewrite in_filter. intros [? Hin]; auto.
+Qed. 
+
+Lemma remove_list_sublist {A: Type} (k: key) (l: list (key * A)) :
+  Common.sublist (remove_list k l) l.
+Proof. apply filter_sublist. Qed.
+
+Lemma map_fst_remove {A: Type} (k: key) (l: list (key * A)) :
+  map fst (remove_list k l) = List.filter (fun x => negb (T.equal k x)) (map fst l).
+Proof.
+  unfold remove_list.
+  induction l as [| h t IH]; simpl; auto.
+  unfold key in *. destruct (T.equal k h.1) eqn : Hkh; simpl; auto.
+  f_equal; auto.
+Qed.
+
+
+Lemma find_ext {A: Type} (p1 p2: A -> bool) (Hp: forall x, p1 x = p2 x) l:
+  find p1 l = find p2 l.
+Proof. 
+  induction l as [| h1 t1 IH]; simpl; auto. rewrite Hp. destruct (p2 h1); auto.
+Qed.
+
+Lemma find_const_r {A: Type} (p: A -> bool) (b1: bool) (l: list A):
+  find (fun x => p x && b1) l = if b1 then find (fun x => p x) l else None.
+Proof.
+  destruct b1.
+  - apply find_ext. intros. apply andb_true_r.
+  - apply find_none_iff. intros x. rewrite andb_false_r. auto.
+Qed. 
+
+Lemma get_list_remove {A: Type} (k: key) (l: list (key * A)) k1 v1:
+  get_list k1 (remove_list k l) = Some v1 <->
+  get_list k1 l = Some v1 /\ negb (T.equal k1 k).
+Proof.
+  unfold remove_list, get_list. rewrite find_filter.
+  rewrite (find_ext _ (fun x => T.equal k1 x.1 && negb (T.equal k1 k))).
+  2: {
+    intros x. destruct (T.equal k1 x.1) eqn : Heq; simpl; auto.
+    destruct (T.equal k x.1) eqn : Heq1;
+    destruct (T.equal k1 k) eqn : Heq2; simpl; auto.
+    - rewrite <- Heq2. apply (T.eq_trans k1 x.1 k); auto. rewrite T.eq_sym; auto.
+    - rewrite <- Heq1. symmetry. apply (T.eq_trans k k1 x.1); auto. rewrite T.eq_sym; auto.
+  }
+  rewrite find_const_r.
+  destruct (T.equal k1 k) eqn : Hkk1; simpl; split; intros; destruct_all; auto; discriminate.
+Qed.
+
+(*TODO: move*)
+Lemma sublist_Forall {A: Type} (P: A -> Prop) (l1 l2: list A):
+  Forall P l2 ->
+  Common.sublist l1 l2 ->
+  Forall P l1.
+Proof.
+  rewrite !List.Forall_forall. unfold Common.sublist. auto.
+Qed.
+
+(*All our specs are in terms of [find_opt]*)
+Definition find_opt {A: Type} (k: key) (m: t A) : option A :=
+  match (mp m) !! tag k with
+  | None => None
+  | Some l => get_list k l
+  end.
+
+(*TODO: fix: also search for key*)
+Definition mem {A: Type} (k: key) (m: t A) : bool :=
+  isSome (find_opt k m).
+
+(*Invariant: only one occurence of key at a time*)
+Definition add_aux {A: Type} (k: key) (v: A) (m: t A) : Zmap (list (key * A)):=
+  <[tag k := (k, v) :: 
+    match (mp m) !! tag k with
+    | None => nil
+    | Some l => remove_list k l
+    end]> (mp m).
+  (* match (mp m) !! tag k with
+  | None => <[tag k :=[(k, v)]]> (mp m)
+  | Some l => <[tag k := (k, v) :: remove_list k l]> (mp m)
+  end. *)
+
+Lemma add_wf {A: Type} (k: key) (v: A) (m: t A):
+  gmap_wf (add_aux k v m).
+Proof.
+  apply gmap_wf_iff. unfold add_aux. destruct m as [m m_wf]; simpl.
+  apply map_Forall_insert_2; [| apply gmap_wf_iff; auto].
+  split; auto. split.
+  - simpl. destruct (m !! tag k) eqn : Hk; auto.
+    rewrite map_fst_remove.
+    rewrite (inb_filter _ T.eq_sym).
+    2: { (*TODO: prove somewhere else once and for all*)
+      intros x y Heq Hneq. destruct (T.equal k y) eqn : Heq2; auto.
+      assert (Heq3: T.equal k x). {
+        apply (T.eq_trans k y x); auto. rewrite T.eq_sym; auto.
+    } unfold is_true in Heq3. rewrite Heq3 in Hneq. discriminate. }
+    rewrite T.eq_refl, andb_false_r; simpl.
+    apply uniq_filter.  apply gmap_wf_iff in m_wf. rewrite map_Forall_lookup in m_wf.
+    specialize (m_wf _ _ Hk); apply m_wf.
+  - constructor; auto.
+    destruct (m !! tag k) eqn : Hk; auto.
+    apply sublist_Forall with (l2:=l); [| apply remove_list_sublist].
+    apply gmap_wf_iff in m_wf. rewrite map_Forall_lookup in m_wf.
+    apply m_wf; auto.
+Qed. 
+
 (*TODO: inline*)
-Definition build_wf {A: Type} {m: Zmap (key * A)} (m_wf: gmap_wf m) : t A :=
+Definition build_wf {A: Type} {m: Zmap (list (key * A))} (m_wf: gmap_wf m) : t A :=
   exist _ m m_wf.
 
 Definition add {a: Type} (k: key) (v: a) (m: t a) : t a :=
   build_wf (add_wf k v m).
 
-Lemma singleton_wf (k: key) (v: a): gmap_wf {[tag k:=(k, v)]}.
+(*And the spec*)
+Lemma add_spec {A: Type} (k1: key) (v1: A) (m: t A) (k: key) (v: A):
+  find_opt k (add k1 v1 m) = Some v <->
+  (T.equal k k1 /\ v = v1) \/ (negb (T.equal k k1) /\ find_opt k m = Some v).
+Proof.
+  unfold find_opt, add. simpl.
+  unfold add_aux.
+  destruct m as [m m_wf]; simpl.
+  destruct (Z.eq_dec (tag k1) (tag k)) as [Heqk | Heqk].
+  - rewrite Heqk, lookup_insert, get_list_cons. simpl.
+    destruct (T.equal k k1) eqn : Hkk1.
+    { split; intros; destruct_all; subst; auto; try discriminate. inversion H; auto. }
+    destruct (m !! tag k) as [l1|] eqn : Hk. 
+    2: { rewrite get_list_nil. split; intros; destruct_all; discriminate. }
+    rewrite get_list_remove. rewrite Hkk1. simpl.
+    split; intros; destruct_all; auto; discriminate.
+  - rewrite lookup_insert_ne; auto.
+    destruct (T.equal k k1) eqn : Hkk1.
+    { apply T.eq_compat in Hkk1. unfold tag in Heqk. rewrite Hkk1 in Heqk.
+      contradiction. }
+    simpl.
+    destruct (m !! tag k) as [l1 |] eqn : Hk; split; intros; destruct_all; auto; discriminate.
+Qed.
+
+Lemma singleton_wf (k: key) (v: a): gmap_wf {[tag k:=[(k, v)]]}.
 Proof.
   apply gmap_wf_iff.
   apply map_Forall_singleton.
-  reflexivity.
+  constructor; auto.
 Qed.
 
 Definition singleton (k: key) (v: a) : t a :=
   build_wf (singleton_wf k v).
 
-Lemma remove_wf (k: key) (m: t a) : 
-  gmap_wf (delete (tag k) (mp m)).
+Lemma singleton_spec (k: key) (v: a) (k1: key) (v1: a) :
+  find_opt k (singleton k1 v1) = Some v <-> T.equal k k1 /\ v = v1.
 Proof.
-  apply gmap_wf_iff, map_Forall_delete, gmap_wf_iff.
-  destruct m; auto.
+  unfold singleton, find_opt. simpl. 
+  destruct (Z.eq_dec (tag k) (tag k1)) as [Htag | Htag].
+  - rewrite Htag, lookup_singleton, get_list_cons, get_list_nil; simpl.
+    destruct (T.equal k k1); split; intros; destruct_all; subst; auto; try discriminate.
+    inversion H; auto.
+  - rewrite lookup_singleton_ne; auto. split; [discriminate|].
+    intros [Heq Hv].
+    apply T.eq_compat in Heq. unfold tag in Htag. rewrite Heq in Htag. contradiction.
 Qed.
 
+Definition remove_aux {A: Type} (k: key) (m: t A) : Zmap (list (key * A)) :=
+  match (mp m) !! tag k with
+  | None => mp m
+  | Some l => let l1 := remove_list k l in
+    if null l1 then delete (tag k) (mp m) else <[tag k := l1]> (mp m)
+  end.
+
+Lemma null_false {A: Type} (l: list A):
+  null l = false <-> l <> nil.
+Proof. destruct l; split; auto. contradiction. Qed.
+
+Lemma remove_wf {A: Type} (k: key) (m: t A):
+  gmap_wf (remove_aux k m).
+Proof.
+  apply gmap_wf_iff. unfold remove_aux.
+  destruct m as [m m_wf]; simpl.
+  destruct (m !! tag k) eqn : Hk; [| apply gmap_wf_iff; auto].
+  destruct (null (remove_list k l)) eqn : Hrem.
+  - apply map_Forall_delete, gmap_wf_iff. auto.
+  - apply map_Forall_insert_2; [| apply gmap_wf_iff; auto].
+    split; [apply null_false; auto |].
+    split.
+    + rewrite map_fst_remove. apply uniq_filter.
+      apply gmap_wf_iff in m_wf. rewrite map_Forall_lookup in m_wf.
+      apply (m_wf _ _ Hk).
+    + apply sublist_Forall with (l2:=l); [| apply remove_list_sublist].
+      apply gmap_wf_iff in m_wf. rewrite map_Forall_lookup in m_wf.
+      apply m_wf; auto.
+Qed.
 
 Definition remove (k: key) (m: t a) : t a :=
   build_wf (remove_wf k m).
+
+(*The spec*)
+Lemma remove_spec (k: key) (v: a) (k1: key) (m: t a) :
+  find_opt k (remove k1 m) = Some v <->
+  (*TODO: equal false or negb?*)
+  negb (T.equal k k1) /\ find_opt k m = Some v.
+Proof.
+  unfold remove, find_opt; simpl.
+  destruct m as [m m_wf]; auto.
+  unfold remove_aux; simpl. unfold key in *.
+  destruct (Z.eq_dec (tag k) (tag k1)) as [Htag | Htag].
+  - rewrite Htag. destruct (m !! tag k1) as [l1|] eqn : Hmk1.
+    2: { rewrite Hmk1. split; intros; destruct_all; discriminate. }
+    destruct (null (remove_list k1 l1)) eqn : Hnull.
+    + unfold key in *. rewrite Hnull.
+      rewrite lookup_delete. split; [discriminate|].
+      intros [Hneq Hget].
+      assert (Hrem: get_list k (remove_list k1 l1) = Some v) by
+        (apply get_list_remove; auto).
+      apply null_nil in Hnull. rewrite Hnull, get_list_nil in Hrem. discriminate.
+    + unfold key in *; rewrite Hnull.
+      rewrite lookup_insert, get_list_remove. apply and_comm.
+  - destruct (T.equal k k1) eqn : Heq.
+    1: { apply T.eq_compat in Heq. unfold tag in Htag; rewrite Heq in Htag; contradiction. }
+    simpl.
+    (*Bunch of cases*)
+    destruct (m !! tag k1) as [l1 |] eqn : Hmk1.
+    + destruct (null (remove_list k1 l1)) eqn : Hnull; unfold key in *; rewrite Hnull;
+      [rewrite lookup_delete_ne | rewrite lookup_insert_ne]; auto; split; intros;
+      destruct_all; auto.
+    + split; intros; destruct_all; auto.
+Qed.
+
+(*TODO: move*)
+(*NOTE: have to add NoDup to invars I think*)
 
 (*Merge is more complicated (but important).
   Merge (in stdpp) does not include the key; this is why we have
   an awkward encoding storing a key, value pair and enforcing 
   the well-formed invariant.*)
+(*NOTE: this is slow, we really need tags to be near-unique*)
+
+(*Specialize to list so we can prove theorems about it*)
+
+Definition fold_add_if {A B C: Type} (f: A -> option B) (g: A -> B -> C)  (l: list A) :=
+  Common.omap (fun x => Common.option_bind (f x) (fun y => Some (g x y))) l.
+
+
+(* Search Common.omap.
+Locate omap.
+    match f x with
+    | None =>) l
+  fold_right (fun x acc =>
+    match f x with
+    | None => acc
+    | Some y => (g x y) :: acc
+    end) nil l. *)
+
+Lemma fold_add_if_in_iff {A B C: Type} (f: A -> option B) (g: A -> B -> C) (l: list A) (z: C):
+  In z (fold_add_if f g l) <-> exists x y, In x l /\ f x = Some y /\ z = g x y.
+Proof.
+  unfold fold_add_if. rewrite in_omap_iff. split.
+  - intros [x [Hinx Hbnd]]. destruct (f x) as [y|] eqn : Hfx; simpl in Hbnd; inversion Hbnd; subst.
+    eauto.
+  - intros [x [y [Hinx [Hf Hz]]]]; subst. exists x. split; auto. rewrite Hf; auto.
+Qed.
+ 
+Lemma fold_add_if_null {A B C: Type} (f: A -> option B) (g: A -> B -> C) (l: list A) :
+  null (fold_add_if f g l) <-> (forall x, In x l -> f x = None).
+Proof.
+  rewrite null_nil. unfold fold_add_if. rewrite omap_nil.
+  split; intros Hin x Hinx; specialize (Hin _ Hinx).
+  - destruct (f x); auto. discriminate.
+  - rewrite Hin; auto.
+Qed. 
+
+Definition merge_list {A B C: Type} (f: key -> option A -> option B -> option C) 
+  (l1: list (key * A)) (l2: list (key * B)) : list (key * C) :=
+  (*Idea: get all keys in l1 and l2 with no dups, then search for each key to compute new list*)
+  let all_keys := unionb T.equal (map fst l1) (map fst l2) in
+  fold_add_if (fun k => f k (get_list k l1) (get_list k l2))
+    (fun k v => (k, v)) all_keys.
+  (* fold_right (fun k acc =>
+    match f k (get_list k l1) (get_list k l2) with
+    | None => acc
+    | Some v => (k, v) :: acc
+    end) nil all_keys. *)
+
+Definition merge_with_none1 {A B C: Type} (f: key -> option A -> option B -> option C)
+  (l: list (key * A)) : list (key * C) :=
+  fold_add_if (fun kv => f (fst kv) (Some (snd kv)) None) (fun kv v => (fst kv, v)) l.
+
+Definition merge_with_none2 {A B C: Type} (f: key -> option A -> option B -> option C)
+  (l: list (key * B)) : list (key * C) :=
+  merge_with_none1 (fun k o1 o2 => f k o2 o1) l.
+(* 
+Definition merge_with_none1 {A B C: Type} (f: key -> option A -> option B -> option C)
+  (l: list (key * A)) : list (key * C) :=
+  fold_add_if (fun kv => f (fst kv) (Some (snd kv)) None) (fun kv v => (fst kv, v)) l.
+  (* fold_right (fun kv acc =>
+    match f (fst kv) (Some (snd kv)) None with
+    | None => acc
+    | Some v => (fst kv, v) :: acc
+    end) nil l. *)
+
+Definition merge_with_none2 {A B C: Type} (f: key -> option A -> option B -> option C)
+  (l: list (key * B)) : list (key * C) :=
+  fold_add_if (fun kv => f (fst kv) None (Some (snd kv))) (fun kv v => (fst kv, v)) l. *)
+  (* fold_right (fun kv acc =>
+    match f (fst kv) None (Some (snd kv)) with
+    | None => acc
+    | Some v => (fst kv, v) :: acc
+    end) nil l. *)
+
+(*TODO: prove spec (prob in terms of [get_list])*)
+
+(*Idea: have 3 cases:
+  if both some, merge the resulting lists
+  if one some and other none, just run f x None for all x in l
+  if both None, key not present so None
+  But in these cases, can't add empty list, so need to ensure that we only add nonempty lists*)
+Definition list_to_opt {A: Type} (l: list A) : option (list A) :=
+  match l with
+  | nil => None
+  | l => Some l
+  end.
+
+Lemma list_to_opt_eq {A: Type} (l: list A) :
+  list_to_opt l = if null l then None else Some l.
+Proof.
+  destruct l; auto.
+Qed.
+
 Definition merge_aux {a b c: Type} (f: key -> option a -> option b -> option c)
   (m1: t a) (m2: t b) := merge
-    (*NOTE: k1 and k2 are always the same by the correctness of
-      the merge operation and our invariants*)
-    (fun (x: option (key * a)) (y: option (key * b)) =>
-      match x with
-      | Some (k1, v1) => option_map (pair k1) 
-                          (f k1 (Some v1) (option_map snd y))
-      | None => 
-        match y with
-        | Some (k2, v2) => option_map (pair k2)
-                              (f k2 None (Some v2))
-        | _ => None
-        end
-      end
-    ) (mp m1) (mp m2).
+    (fun (x: option (list (key * a))) (y: option (list (key * b))) =>
+      match x, y with
+      | Some l1, Some l2 => list_to_opt (merge_list f l1 l2)
+      | Some l1, None => list_to_opt (merge_with_none1 f l1)
+      | None, Some l2 => list_to_opt (merge_with_none2 f l2)
+      | None, None => None
+      end) (mp m1) (mp m2).
 
+Lemma isSome_get_list {A: Type} k (l: list (key * A)):
+  isSome (get_list k l) = inb T.equal k (map fst l).
+Proof.
+  induction l as [| h1 t1 IH]; auto.
+  rewrite get_list_cons. simpl. destruct (T.equal k h1.1); auto.
+Qed.
+
+Lemma get_list_congr {A: Type} k1 k2 (l: list (key * A)):
+  T.equal k1 k2 ->
+  get_list k1 l = get_list k2 l.
+Proof.
+  intros Heq. induction l as [| h1 t1]; auto.
+  rewrite !get_list_cons.
+  rewrite IHt1.
+  replace (T.equal k1 h1.1) with (T.equal k2 h1.1); auto.
+  destruct (T.equal k1 h1.1) eqn : Heq1; destruct (T.equal k2 h1.1) eqn : Heq2; auto.
+  - rewrite <- Heq2. apply (T.eq_trans k2 k1 h1.1); auto. rewrite T.eq_sym; auto.
+  - rewrite <- Heq1. symmetry. apply (T.eq_trans k1 k2 h1.1); auto.
+Qed.
+
+(*Problem: we have f taking in a key, morally speaking, any two T.equal keys should produce the
+  same f, but this is NOT the case necessarily
+  Example, for terms: f could be: if t contains the variable "x" then Some tt else None
+  then we can have two terms that are alpha-equivalent (T.equal) but merge is not the same
+  what is the behavior of merge supposed to be in this case?
+
+  Alternatively, we could require that equality corresponds to Leibnitz equality for the
+  proof of merge
+
+  Option 3: we can give a less nice spec, something like (need In predicate on maps):
+  find_opt k (merge f m1 m2) = Some v <->
+  exists k1, In k1 m1 \/ In k1 m1 /\ T.equal k k1 /\ f k1 (find_opt k m1) (find_opt k m2) = Some v
+  Is this formulation even useful?
+
+  (nicer way for this third option:)
+  forall k, In k m1 \/ In k m2 ->
+    find_opt k (merge f m1 m2) = f k (find_opt k m1) (find_opt k m2)
+  and
+  (other direction harder, because equivalence)
+  forall k, ~ In k m1 -> ~ In k m2 -> find_opt k 
+
+  easier alternative: impose condition that f respects equality
+  
+  *)
+
+Lemma contra_b {b1: bool} (Hb: b1 = false) : ~ b1.
+Proof. subst. auto. Qed.
+
+Lemma get_list_in_iff {A: Type} (k: key) (v: A) (l: list (key * A)):
+  uniq T.equal (map fst l) ->
+  get_list k l = Some v <-> exists k1, T.equal k k1 /\ In (k1, v) l.
+Proof.
+  induction l as [| [k1 v1] t1 IH]; simpl.
+  - intros _. rewrite get_list_nil. split; intros; destruct_all; try contradiction; discriminate.
+  - intros Huniq. apply andb_true_iff in Huniq. destruct Huniq as [Hnotin Huniq]. 
+    rewrite get_list_cons; simpl. destruct (T.equal k k1) eqn : Heq.
+    + split; [intros Hsome; inversion Hsome; subst; eauto |].
+      intros [k2 [Heq2 [Heq3 | Hin2]]]; [inversion Heq3; subst; auto |].
+      apply negb_true_iff in Hnotin.
+      exfalso. apply (contra_b Hnotin).
+      rewrite (inb_congr _ T.eq_sym T.eq_trans _ k1 k2).
+      2: { apply (T.eq_trans k1 k k2); auto; rewrite T.eq_sym; auto. }
+      apply (In_inb _ T.eq_refl). rewrite in_map_iff. exists (k2, v); auto.
+    + rewrite IH; auto. split; [intros; destruct_all; eauto |].
+      intros [k2 [Heqk [Heq2 | Hin]]]; [inversion Heq2; subst | eauto].
+      exfalso. apply (contra_b Heq); auto.
+Qed.
+
+Lemma get_list_none_iff {A: Type} (k: key) (l: list (key * A)):
+  get_list k l = None <-> negb (inb T.equal k (map fst l)).
+Proof.
+  induction l as [| [k1 v1] t1 IH]; simpl; auto.
+  - rewrite get_list_nil. split; auto.
+  - rewrite get_list_cons; simpl. destruct (T.equal k k1); simpl; auto.
+    split; discriminate.
+Qed.
+
+Lemma merge_list_inb_aux {C: Type} (f: T.t -> option C) (Hf: forall k1 k2, T.equal k1 k2 -> f k1 = f k2) 
+  k l:
+  inb T.equal k (map fst (fold_add_if f (fun k1 v1 => (k1, v1)) l))  = inb T.equal k l && isSome (f k).
+Proof.
+  induction l as [| h1 t1 IH]; simpl; auto.
+  destruct (f h1) eqn : Hfeq; simpl; auto.
+  - destruct (T.equal k h1) eqn : Heq; simpl; auto.
+    rewrite (Hf _ h1); auto. rewrite Hfeq; auto.
+  - rewrite IH. destruct (T.equal k h1) eqn : Heq; simpl; auto.
+    rewrite (Hf k h1); auto. rewrite Hfeq; simpl; rewrite andb_false_r; auto.
+Qed.
+
+(*Weaker unconditional version (TODO: do we need?)*)
+Lemma merge_list_inb_aux' {C: Type} (f: T.t -> option C) k l:
+  inb T.equal k (map fst (fold_add_if f (fun k1 v1 => (k1, v1)) l)) -> inb T.equal k l.
+Proof.
+  induction l as [| h1 t1 IH]; simpl; auto.
+  destruct (f h1) eqn : Hf; simpl; auto.
+  - apply orb_impl_l; auto.
+  - intros Hin. rewrite IH, orb_true_r; auto.
+Qed. 
+
+(* Lemma merge_list_inb_aux {C: Type} (f: T.t -> option C) k l:
+  inb T.equal k (map fst (fold_add_if f (fun k1 v1 => (k1, v1)) l)) -> inb T.equal k l.
+Proof.
+  induction l as [| h1 t1 IH]; simpl; auto.
+  destruct (f h1) eqn : Hf; simpl; auto.
+  - apply orb_impl_l; auto.
+  - intros Hin. rewrite IH, orb_true_r; auto.
+Qed.  *)
+
+Lemma merge_list_inb {A B C: Type} (f: key -> option A -> option B -> option C)
+  (Hf: forall k1 k2 o1 o2, T.equal k1 k2 -> f k1 o1 o2 = f k2 o1 o2) l1 l2 k:
+  inb T.equal k (map fst (merge_list f l1 l2)) = 
+  inb T.equal k (unionb T.equal (map fst l1) (map fst l2)) && isSome (f k (get_list k l1) (get_list k l2)).
+Proof.
+  apply (@merge_list_inb_aux C); intros k1 k2 Heq.
+  rewrite (get_list_congr k1 k2 l1), (get_list_congr k1 k2 l2); auto.
+Qed.
+(* 
+Lemma merge_list_inb {A B C: Type} (f: key -> option A -> option B -> option C) l1 l2 k:
+  inb T.equal k (map fst (merge_list f l1 l2)) -> inb T.equal k (unionb T.equal (map fst l1) (map fst l2)).
+Proof.
+  apply (@merge_list_inb_aux C).
+Qed. *)
+(*NOTE: dont want assumptions on f because we will want for wf*)
+Lemma merge_list_uniq {A B C: Type} (f: key -> option A -> option B -> option C) l1 l2
+  (Huniq: uniq T.equal (map fst l2)):
+  uniq T.equal (map fst (merge_list f l1 l2)).
+Proof.
+  unfold merge_list.
+  assert (Huniqu: uniq T.equal (unionb T.equal (map fst l1) (map fst l2))) by
+    (apply uniq_unionb; auto).
+  clear Huniq. unfold key in *. generalize dependent (unionb T.equal (map fst l1) (map fst l2)).
+  induction l as [| h1 t1 IH]; auto; simpl; intros Huniq.
+  apply andb_true_iff in Huniq. destruct Huniq as [Hnotin Huniq].
+  destruct (f h1 (get_list h1 l1) (get_list h1 l2))eqn : Hf; simpl; auto.
+  apply andb_true_iff; split; auto; [| apply IH; auto].
+  apply eq_true_not_negb. intros Hin.
+  apply merge_list_inb_aux' in Hin.
+  rewrite Hin in Hnotin. discriminate.
+Qed.
+
+(*TODO: what do we need?*)
+
+Lemma merge_with_none1_inb_aux' {A C: Type} (f: (T.t * A) -> option C) k l:
+  inb T.equal k (map fst (fold_add_if f (fun k1 v1 => (k1.1, v1)) l)) -> inb T.equal k (map fst l).
+Proof.
+  induction l as [| h1 t1 IH]; simpl; auto.
+  destruct (f h1) eqn : Hf; simpl; auto.
+  - apply orb_impl_l; auto.
+  - intros Hin. rewrite IH, orb_true_r; auto.
+Qed. 
+
+Lemma merge_with_none1_get {A B C: Type} (f: key -> option A -> option B -> option C)
+  (Hf: forall k1 k2 o1 o2, T.equal k1 k2 -> f k1 o1 o2 = f k2 o1 o2) l
+  (Huniq: uniq T.equal (map fst l)) k
+  :
+    get_list k (merge_with_none1 f l) =
+    match (get_list k l) with
+    | Some v => f k (Some v) None
+    | None => None
+    end.
+Proof.
+  unfold merge_with_none1. induction l as [| [k1 v1] t1 IH]; simpl; auto.
+  rewrite get_list_cons; simpl.
+  simpl in Huniq. apply andb_true_iff in Huniq. destruct Huniq as [Hnotin Huniq].
+  destruct (T.equal k k1) eqn : Heq;
+  destruct (f k1 (Some v1) None) eqn : Hfeq; simpl; auto.
+  - rewrite get_list_cons. simpl. rewrite Heq. 
+    erewrite Hf; eauto.
+  - (*[get_list] is None because k not in t1*)
+    replace (get_list k _) with (@None C); [erewrite Hf; eauto|].
+    symmetry. apply get_list_none_iff.
+    apply eq_true_not_negb; intros Hin. apply merge_with_none1_inb_aux'  in Hin.
+    rewrite (inb_congr _ T.eq_sym T.eq_trans _ k k1) in Hin by auto.
+    rewrite Hin in Hnotin; discriminate.
+  - (*Not equal, get_list is Some (IH)*)
+    rewrite get_list_cons; simpl. rewrite Heq. auto.
+Qed.
+
+Lemma merge_with_none1_uniq {A B C: Type} (f: key -> option A -> option B -> option C) l1
+  (Huniq: uniq T.equal (map fst l1)):
+  uniq T.equal (map fst (merge_with_none1 f l1)).
+Proof.
+  unfold merge_with_none1.
+  unfold key in *. induction l1 as [| h1 t1 IH]; simpl; auto.
+  simpl in Huniq. apply andb_true_iff in Huniq. destruct Huniq as [Hnotin Huniq].
+  destruct (f h1.1 (Some h1.2) None) eqn : Hf; simpl; auto.
+  apply andb_true_iff; split; [| apply IH; auto].
+  apply eq_true_not_negb. intros Hin.
+  apply merge_with_none1_inb_aux' in Hin. rewrite Hin in Hnotin; discriminate.
+Qed.
+
+Lemma isSome_get_list_union {A B: Type} (l1: list (key * A)) (l2: list (key * B)) k:
+  isSome (get_list k l1) || isSome (get_list k l2) = 
+  inb T.equal k (unionb T.equal (map fst l1) (map fst l2)).
+Proof.
+  rewrite !isSome_get_list, inb_unionb; auto.
+  - apply T.eq_sym.
+  - apply T.eq_trans.
+Qed.
+(* Check gmap_wf_iff.*)
+Lemma map_get_wf {A: Type} {m: Zmap (list (key * A))} {k: key} {l1}
+  (Hwf: gmap_wf m) (Hin: m !! tag k = Some l1):
+  l1 <> nil /\ uniq T.equal (map fst l1) /\ Forall (fun x => tag k = tag x.1) l1.
+Proof.
+  apply gmap_wf_iff in Hwf. rewrite map_Forall_lookup in Hwf.
+  apply Hwf; auto.
+Qed.
+
+Lemma tag_cond_alt {A: Type} k (l: list (key * A)):
+  Forall (fun x => k = tag (fst x)) l <->
+  Forall (fun x => k = tag x) (map fst l).
+Proof.
+  rewrite Forall_map; auto.
+Qed.
+
+(*Prove merge wf*)
 Lemma merge_aux_wf {A B C: Type} (f: key -> option A -> option B -> option C)
   (m1: t A) (m2: t B) : gmap_wf (merge_aux f m1 m2).
 Proof.
-  unfold merge_aux.
-  apply gmap_wf_iff.
+  apply gmap_wf_iff. unfold merge_aux. destruct m1 as [m1 m1_wf]; simpl.
+  destruct m2 as [m2 m2_wf]; simpl.
   (*Need to use definition*)
   unfold map_Forall.
   intros k v.
   rewrite lookup_merge.
   unfold diag_None.
-  destruct m1 as [m1 m1_wf].
-  destruct m2 as [m2 m2_wf].
-  simpl.
   apply gmap_wf_iff in m1_wf, m2_wf.
   unfold map_Forall in m1_wf, m2_wf.
   destruct (m1 !! k) as [v1|] eqn : Hm1k.
   - apply m1_wf in Hm1k; subst.
-    destruct v1 as [k1 a1]; simpl.
-    unfold option_map.
-    destruct (m2 !! tag k1) as [v1|] eqn : Hm2k.
-    + apply m2_wf in Hm2k. subst.
-      destruct (f _ _ _); [|discriminate].
-      intros Heq; inversion Heq; subst; reflexivity.
-    + destruct (f _ _ _); [|discriminate].
-      intros Heq; inversion Heq; subst; reflexivity.
-  - destruct (m2 !! k) as [v2|] eqn : Hm2k; [|discriminate].
-    apply m2_wf in Hm2k; subst.
-    destruct v2 as [k2 a2]; simpl in *.
-    unfold option_map.
-    destruct (f _ _ _); [|discriminate].
-    intros Heq; inversion Heq; subst; auto.
+    destruct (m2 !! k) as [v2|] eqn : Hm2k.
+    + apply m2_wf in Hm2k.
+      intros Hmerge.
+      rewrite list_to_opt_eq in Hmerge.
+      destruct (null (merge_list f v1 v2)) eqn : Hnull; [discriminate|].
+      inversion Hmerge; subst; clear Hmerge.
+      split; [apply null_false; auto |].
+      split; [apply merge_list_uniq; apply Hm2k |].
+      (*rewrite tag_cond_alt.*)
+      rewrite List.Forall_forall. intros x Hinx.
+      (*Can't use [merge_list_inb] because we don't want to assume anything about f*)
+      unfold merge_list in Hinx.
+      rewrite fold_add_if_in_iff in Hinx.
+      destruct Hinx as [k3 [v3 [Hink3 [Hfk Hy]]]]; subst. simpl.
+      (*Now deal with In/inb*)
+      apply In_inb with (eq:=T.equal) in Hink3; [| apply T.eq_refl].
+      rewrite inb_unionb in Hink3; [| apply T.eq_sym | apply T.eq_trans].
+      (*Very annoying - have to go back to In*)
+      assert (Htageq: forall (A: Type) (l: list (key * A)), 
+        inb T.equal k3 (map fst l) -> Forall (fun x => k = tag x.1) l ->
+        k = tag k3).
+      {
+        clear Hink3 Hnull Hfk. intros T l Hin Hall.
+        destruct (inb_In _ _ _ Hin) as [k4 [Hink4 Heq]].
+        rewrite tag_cond_alt in Hall.
+        rewrite List.Forall_forall in Hall.
+        apply Hall in Hink4. subst. unfold tag. f_equal. apply T.eq_compat. 
+        rewrite T.eq_sym; auto.
+      }
+      apply orb_true_iff in Hink3; destruct Hink3 as [Hink3 | Hink3]; 
+      apply (Htageq _ _ Hink3); [apply Hm1k | apply Hm2k].
+    + (*first some, second None*)
+      rewrite list_to_opt_eq.
+      destruct (null (merge_with_none1 _ v1)) eqn : Hnull; [discriminate|].
+      intros Hsome; inversion Hsome; subst; clear Hsome.
+      split; [apply null_false; auto |].
+      split; [apply merge_with_none1_uniq; apply Hm1k |].
+      rewrite List.Forall_forall. intros x Hinx.
+      unfold merge_with_none1 in Hinx.
+      rewrite fold_add_if_in_iff in Hinx.
+      destruct Hinx as [k3 [v3 [Hink3 [Hfk Hy]]]]; subst. simpl.
+      destruct Hm1k as [_ [_ Hall]]. rewrite List.Forall_forall in Hall.
+      apply Hall in Hink3. auto.
+  - destruct (m2 !! k) as [v1 |] eqn : Hm2k; [|discriminate].
+    (*similar to previous case*)
+    apply m2_wf in Hm2k.
+    rewrite list_to_opt_eq. unfold merge_with_none2.
+    destruct (null (merge_with_none1 _ v1)) eqn : Hnull; [discriminate|].
+    intros Hsome; inversion Hsome; subst; clear Hsome.
+    split; [apply null_false; auto |].
+    split; [apply merge_with_none1_uniq; apply Hm2k |].
+    rewrite List.Forall_forall. intros x Hinx.
+    unfold merge_with_none1 in Hinx.
+    rewrite fold_add_if_in_iff in Hinx.
+    destruct Hinx as [k3 [v3 [Hink3 [Hfk Hy]]]]; subst. simpl.
+    destruct Hm2k as [_ [_ Hall]]. rewrite List.Forall_forall in Hall.
+    apply Hall in Hink3. auto.
 Qed.
 
 Definition merge {a b c: Type} (f: key -> option a -> option b -> option c)
   (m1: t a) (m2: t b) : t c := build_wf (merge_aux_wf f m1 m2).
+
+(*Merge is complicated to prove correct (unsurprisingly, as it is the crucial operation)*)
+Lemma merge_spec {A B C: Type} (f: key -> option A -> option B -> option C)
+  (*if f doesn't respect equality, things get very complicated*)
+  (Hf: forall k1 k2 o1 o2, T.equal k1 k2 -> f k1 o1 o2 = f k2 o1 o2) 
+  (m1: t A) (m2: t B) k:
+  (*The spec is pretty element: for all keys in 1, the value is f on the results*)
+  find_opt k (merge f m1 m2) = 
+    if (mem k m1 || mem k m2) then
+    f k (find_opt k m1) (find_opt k m2) 
+    else None.
+Proof.
+  unfold merge, mem,find_opt, merge_aux. simpl.
+  destruct m1 as [m1 m1_wf]; destruct m2 as [m2 m2_wf]; simpl.
+  rewrite lookup_merge.
+  destruct (m1 !! tag k) as [l1 |] eqn : Hm1k; destruct (m2 !! tag k) as [l2 |] eqn : Hm2k; simpl; auto.
+  - (*Case 1: in both lists*)
+    rewrite list_to_opt_eq.
+    destruct (null (merge_list f l1 l2)) eqn : Hnull.
+    + unfold merge_list in Hnull.
+      rewrite fold_is_true in Hnull.
+      rewrite fold_add_if_null in Hnull.
+      destruct_if Hsome; auto.
+      (*A bit annoying because we have 2 inequivalent notions of "in"*)
+      assert (Hin1: inb T.equal k (unionb T.equal (map fst l1) (map fst l2))).
+      { rewrite (inb_unionb _ T.eq_sym T.eq_trans).
+        rewrite !isSome_get_list in Hsome. auto.
+      }
+      destruct (inb_In _ _ _ Hin1) as [k1 [Hink1 Heqk]].
+      specialize (Hnull _ Hink1). symmetry.
+      erewrite (get_list_congr _ _ l2), (get_list_congr _ _ l1); [ rewrite (Hf _ _ _ _ Heqk); apply Hnull | auto | auto].
+    + (*Interesting case - merge both lists*) destruct (get_list k _) as [v1|] eqn : Hget.
+      * (*Some case*)
+        rewrite get_list_in_iff in Hget.
+        2: {
+          (*Need to prove uniqueness of [merge_list]*)
+          apply merge_list_uniq.
+          apply (map_get_wf m2_wf Hm2k).
+        }
+        destruct Hget as [k1 [Heqk Hinmerge]].
+        unfold merge_list in Hinmerge.
+        apply fold_add_if_in_iff in Hinmerge.
+        destruct Hinmerge as [k3 [v3 [Hinu [Hfeq Htup]]]]; inversion Htup; subst; auto; clear Htup.
+        (*Now we need to know that the [isSome] part holds*)
+        rewrite isSome_get_list_union.
+        pose proof (In_inb _ T.eq_refl _ _ Hinu) as Hink3.
+        rewrite inb_congr with (x2:=k3); auto; [| apply T.eq_sym | apply T.eq_trans].
+        rewrite Hink3. symmetry.
+        rewrite (Hf _ k3); auto.
+        rewrite (get_list_congr _ k3 l1), (get_list_congr _ k3 l2); auto.
+      * (*None case*)
+        rewrite get_list_none_iff in Hget.
+        rewrite merge_list_inb in Hget; auto.
+        rewrite inb_unionb in Hget; [| apply T.eq_sym | apply T.eq_trans].
+        rewrite negb_andb in Hget.
+        rewrite !isSome_get_list. apply orb_true_iff in Hget; destruct Hget as [Hnotin | Hnone].
+        -- apply negb_true_iff in Hnotin. rewrite Hnotin. auto.
+        -- destruct (_ || _); auto.
+            destruct (f k (get_list k l1) (get_list k l2)); auto. discriminate. 
+  - (*Case 2: In left list only*)
+    rewrite list_to_opt_eq.
+    destruct (null (merge_with_none1 f l1)) eqn : Hnull.
+    + unfold merge_with_none1 in Hnull.
+      rewrite fold_is_true in Hnull.
+      rewrite fold_add_if_null in Hnull.
+      rewrite orb_false_r.
+      (*Again deal with In vs inb*)
+      destruct (get_list k l1) as [v|] eqn : Hget; auto.
+      rewrite get_list_in_iff in Hget.
+      2: apply (map_get_wf m1_wf Hm1k).
+      simpl.
+      destruct Hget as [k1 [Hkeq Hink1]].
+      apply Hnull in Hink1; simpl in *.
+      rewrite (Hf _ _ _ _ Hkeq); auto.
+    + (*merge single list with None*)
+      rewrite orb_false_r.
+      destruct (get_list k (merge_with_none1 f l1)) as [v|] eqn : Hget.
+      * rewrite get_list_in_iff in Hget by (apply merge_with_none1_uniq, (map_get_wf m1_wf Hm1k)).
+        destruct Hget as [k1 [Heqk Hink]].
+        unfold merge_with_none1 in Hink.
+        apply fold_add_if_in_iff in Hink.
+        destruct Hink as [k3 [v3 [Hinu [Hfeq Htup]]]]; inversion Htup; subst; auto; clear Htup.
+        (*Prove that [get_list] holds*)
+        rewrite isSome_get_list.
+        rewrite (inb_congr _ T.eq_sym T.eq_trans _ k k3.1); auto.
+        rewrite (In_inb _ T.eq_refl). 2: { rewrite in_map_iff; exists k3; destruct k3; auto. }
+        (*Now prove that [get_list k l1] = Some k3.3*)
+        replace (get_list k l1) with (Some k3.2).
+        -- symmetry. erewrite Hf; eauto.
+        -- symmetry. apply get_list_in_iff; [apply (map_get_wf m1_wf Hm1k)|].
+          exists k3.1; auto. destruct k3; auto.
+      * (*Not in merge*)
+        rewrite get_list_none_iff in Hget.
+        rewrite <- isSome_get_list in Hget.
+        rewrite merge_with_none1_get in Hget; [ | auto | apply (map_get_wf m1_wf Hm1k)].
+        destruct (get_list k l1) as [v1 |] eqn : Hget1; auto. simpl.
+        destruct (f k (Some v1) None); auto; discriminate.
+  - (*Case 3: In right left only (very similar)*)
+    rewrite list_to_opt_eq. unfold merge_with_none2.
+    destruct (null (merge_with_none1 _ l2)) eqn : Hnull.
+    + unfold merge_with_none1 in Hnull.
+      rewrite fold_is_true in Hnull.
+      rewrite fold_add_if_null in Hnull.
+      (*Again deal with In vs inb*)
+      destruct (get_list k l2) as [v|] eqn : Hget; auto.
+      rewrite get_list_in_iff in Hget.
+      2: apply (map_get_wf m2_wf Hm2k).
+      simpl.
+      destruct Hget as [k1 [Hkeq Hink1]].
+      apply Hnull in Hink1; simpl in *.
+      rewrite (Hf _ _ _ _ Hkeq); auto.
+    + (*merge single list with None*)
+      destruct (get_list k (merge_with_none1 _ l2)) as [v|] eqn : Hget.
+      * rewrite get_list_in_iff in Hget by (apply merge_with_none1_uniq, (map_get_wf m2_wf Hm2k)).
+        destruct Hget as [k1 [Heqk Hink]].
+        unfold merge_with_none1 in Hink.
+        apply fold_add_if_in_iff in Hink.
+        destruct Hink as [k3 [v3 [Hinu [Hfeq Htup]]]]; inversion Htup; subst; auto; clear Htup.
+        (*Prove that [get_list] holds*)
+        rewrite isSome_get_list.
+        rewrite (inb_congr _ T.eq_sym T.eq_trans _ k k3.1); auto.
+        rewrite (In_inb _ T.eq_refl). 2: { rewrite in_map_iff; exists k3; destruct k3; auto. }
+        replace (get_list k l2) with (Some k3.2).
+        -- symmetry. erewrite Hf; eauto.
+        -- symmetry. apply get_list_in_iff; [apply (map_get_wf m2_wf Hm2k)|].
+          exists k3.1; auto. destruct k3; auto.
+      * (*Not in merge*)
+        rewrite get_list_none_iff in Hget.
+        rewrite <- isSome_get_list in Hget.
+        rewrite merge_with_none1_get in Hget; [ | auto | apply (map_get_wf m2_wf Hm2k)].
+        destruct (get_list k l2) as [v1 |] eqn : Hget1; auto. simpl.
+        destruct (f k None (Some v1)); auto; discriminate.
+Qed.
+
 
 (*Follow OCaml spec of union in terms of merge*)
 Definition union (f: key -> a -> a -> option a) (m1: t a) (m2: t a):
@@ -852,5 +1703,62 @@ Definition start_ge_enum {A: Type} (k: key) (m: t A) : enumeration A :=
   next_ge_enum k (start_enum m).
 
 Definition test := 0%nat.
+
+
+(*Lemmas*)
+
+(*Need merge spec*)
+
+Lemma merge_spec: forall {a b c: Type} (f: key -> option a -> option b -> option c) (m1: t a) (m2: t b)
+  (k: key),
+  find_opt _ k (merge f m1 m2) = f k (find_opt _ k m1) (find_opt _ k m2).
+Proof.
+  intros a b c f m1 m2 k.
+  unfold merge, find_opt. simpl.
+  unfold merge_aux.
+  destruct m1 as [m1 m1_wf]; destruct m2 as [m2 m2_wf]; simpl.
+  rewrite lookup_merge.
+  unfold diag_None.
+  destruct (m1 !! tag k) as [[k1 v1] |] eqn : Hm1k; simpl.
+  - assert (Htag: tag k = tag k1). {
+      apply gmap_wf_iff in m1_wf.
+      eapply map_Forall_lookup_1 in m1_wf. 2: apply Hm1k. auto.
+   }
+   destruct (m2 !! tag k) as [[k2 v2] |] eqn : Hm2k; simpl.
+    + unfold option_map; simpl. destruct (f k (Some v1) (Some v2)) eqn : Hf; simpl.
+
+   unfold option_map.  simpl. 
+  
+   simpl.
+  rewrite zmap.Zmap_lookup_merge.
+  unfold base.merge.
+  Search Zmap_merge.
+  rewrite (pmap.Pmap_lookup_merge _ m1 m2 (tag k)).
+  
+   Search base.merge. Locate base.merge.
+
+
+  pmap.Pmap_lookup_merge:
+  ∀ {A B C : Type} (f : option A → option B → option C) 
+    (mt1 : Pmap A) (mt2 : Pmap B) (i : positive),
+    base.merge f mt1 mt2 !! i = diag_None f (mt1 !! i) (mt2 !! i)
+  
+  
+  . base.merge. simpl.
+
+  unfold find_opt.
+   = Some v
+
+Lemma find_opt_inter: forall {a b c: Type} (f: key -> a -> b -> option c) (m1: t a) (m2: t b)
+  (k: key) (v: c),
+  find_opt _ k (inter f m1 m2) = Some v <-> 
+  exists v1 v2, find_opt _ k m1 = Some v1 /\ find_opt _ k m2 = Some v2 /\ f k v1 v2 = Some v.
+Proof.
+  intros a b c f m1 m2 k v.
+  unfold inter.
+
+Parameter find_opt_set_inter: forall {a: Type} (m1 m2: t a) (k: key) (v: a),
+  find_opt k (set_inter m1 m2) = Some v <->
+  find_opt k m1 = Some v /\ exists v2, find_opt k m2 = Some v2.
 
 End Make.
